Adam-style transactional disk
The high-level language tprog operates on two hypothetical disks:
one for normal read/writes (nx-disk), the other (alt-disk) for
read/writes inside a transaction.

TBegin copies nx-disk to alt-disk; writes inside a transaction
are made on the alt-disk (i.e. isolation); TEnd replace nx-disk
with the content of alt-disk (i.e. atomicity). The correctness
of this level is easy to verify --- if tprog halts inside a
transaction, the nx-disk is left intact.

This abstraction can be easily extended to support multiple
transactions, by introducing multiple alt-disks organized as
a stack (for nested tx) or a map (for concurrent tx).

The low-level language pprog implement the alt-disk with an
in-memory pending list and a tx flag. Primitives to access them
include GetLog, GetTx, AddLog, ClrLog and SetTx. We choose these
fine-grained operations so that during further refinement, they
can be implmented in the lower level with real disks efficiently.

pprog level could crash, for now it halts after running the
recovery procedure (which we assume does not fail).
In real world, we want the system to continue running after recovery,
and the recovery procedure could fail too. Maybe we can model this
by simply changing the stepping rule (PsCrash)?

src/Fs9.v
@@ -6,122 +6,223 @@ Set Implicit Arguments.
 
 Definition value := nat.
 Definition block := nat.
-Definition trans := nat.
 
 Parameter storage : Set.
-Parameter st_init  : storage.
 Parameter st_write : storage -> block -> value -> storage.
 Parameter st_read  : storage -> block -> value.
-Parameter st_fail  : storage -> bool.
 
-(* high-level language *)
+(** high-level language for a transactional disk *)
 
-Inductive TOp : Set :=
-  | TRead:  block -> TOp
-  | TWrite: block -> value -> TOp
-  | TBegin: trans -> TOp
-  | TEnd:   trans -> TOp
+(* return values *)
+Inductive trs :=
+  | TRValue (v:value)
+  | TRSucc
+  | TRFail
   .
 
-Inductive TResult : Set :=
-  | TRValue: value -> TResult
-  | TRNone: TResult
-  | TRSucc: TResult
-  | TRFail: TResult
-  | TRCrash: TResult
+Inductive tprog :=
+  | TRead  (b:block) (rx:trs -> tprog)
+  | TWrite (b:block) ( v:value) (rx:trs -> tprog)
+  | TBegin (rx:trs -> tprog)
+  | TEnd   (rx:trs -> tprog)
+  | THalt
   .
 
-Record TState: Set := mkTState {
-  disk : storage;
-  result : TResult;                (* result of last invocation *)
-  intrans : bool;
-  pending : list (block * value)   (* list of pending writes in a transaction *)
+Record tstate := TSt {
+  TSDisk: storage;            (* main disk *)
+  TSAltDisk: option storage   (* alternative disk for transactions *)
 }.
 
-Definition TProg := list TOp.
+(* high level interpreter *)
+Fixpoint texec (p:tprog) (s:tstate) : tstate :=
+  let (d, ad) := s in
+  match p with
+  | THalt         => s
+  | TRead b rx    =>
+    match ad with
+    | None   => texec (rx (TRValue (st_read d b))) (TSt d ad)
+    | Some x => texec (rx (TRValue (st_read x b))) (TSt d ad)
+    end
+  | TWrite b v rx =>
+    match ad with
+    | None   => texec (rx TRSucc) (TSt (st_write d b v) ad)
+    | Some x => texec (rx TRSucc) (TSt d (Some (st_write x b v)))
+    end
+  | TBegin rx     =>
+    match ad with
+    | None   => texec (rx TRSucc) (TSt d (Some d))
+    | Some _ => texec (rx TRFail) (TSt d ad)
+    end
+  | TEnd rx       =>
+    match ad with
+    | Some d => texec (rx TRSucc) (TSt d None)
+    | None   => texec (rx TRFail) (TSt d ad)
+    end
+  end
+.
 
-Fixpoint Tfind_pending (p:list (block * value)) (b:block) : option value :=
+
+(* language that manipulates a disk and an in-memory pending log *)
+
+Inductive pprog :=
+  | PRead   (b:block) (rx:value -> pprog)
+  | PWrite  (b:block) ( v:value) (rx:pprog)
+  | PAddLog (b:block) ( v:value) (rx:pprog)
+  | PClrLog (rx:pprog)
+  | PGetLog (rx:list (block * value) -> pprog)
+  | PSetTx  (v:bool) (rx:pprog)
+  | PGetTx  (rx:bool -> pprog)
+  | PHalt
+  .
+
+Record pstate := PSt {
+  PSDisk: storage;
+  PSLog: list (block * value);
+  PSTx: bool
+}.
+
+Bind Scope pprog_scope with pprog.
+
+Notation "ra <- a ; b" := (a (fun ra => b))
+  (right associativity, at level 60) : pprog_scope.
+
+Notation "a ;; b" := (a (b))
+  (right associativity, at level 60) : pprog_scope.
+
+Open Scope pprog_scope.
+
+Fixpoint pfind (p:list (block * value)) (b:block) : option value :=
   match p with
   | nil => None
   | (b', v) :: rest =>
-    if eq_nat_dec b b' then Some v else Tfind_pending rest b
+    match (pfind rest b) with
+    | None => if eq_nat_dec b b' then Some v else None
+    | x    => x
+    end
   end.
 
-Fixpoint Tcommit (s:storage) (p:list (block*value)): storage :=
+Fixpoint pflush (p:list (block*value)) rx : pprog :=
   match p with
-  | nil => s
-  | (b, v) :: rest =>
-      let s' := Tcommit s rest in st_write s' b v
+  | nil            => rx
+  | (b, v) :: rest => PWrite b v ;; pflush rest rx
   end.
 
-Inductive Tstep : TState -> TState -> Prop :=
-  | TRead_ex_tx:
-      forall d r p b, r <> TRCrash ->
-      let r' := match (Tfind_pending p b) with
-      | Some v => TRValue v
-      | None   => TRValue (st_read d b)
-      end in
-      Tstep (mkTState d r true p) (mkTState d r' true p)
-  | TRead_ex:
-      forall d r p b, r <> TRCrash ->
-      let r' := TRValue (st_read d b) in
-      Tstep (mkTState d r false p) (mkTState d r' false p)
-  | TWrite_ex_tx:
-      forall d r p b v, r <> TRCrash ->
-      Tstep (mkTState d r true p)  (mkTState d TRSucc true ((b, v) :: p))
-  | TWrite_ex:
-      forall d r p, r <> TRCrash ->
-      Tstep (mkTState d r false p) (mkTState d TRFail false p)
-  | TBegin_ex_tx:
-      forall d r p, r <> TRCrash ->
-      Tstep (mkTState d r true p)  (mkTState d TRFail true p)
-  | TBegin_ex:
-      forall d r p, r <> TRCrash ->
-      Tstep (mkTState d r false p) (mkTState d TRSucc true nil)
-  | TEnd_ex_tx:
-      forall d r p, r <> TRCrash ->
-      let d' := Tcommit d p in
-      Tstep (mkTState d r true p)  (mkTState d' TRSucc false nil)
-  | TEnd_ex:
-      forall d r p, r <> TRCrash ->
-      Tstep (mkTState d r false p) (mkTState d TRFail false p)
-  | TCrash:
-      forall d r tx p,
-      Tstep (mkTState d r tx p) (mkTState d TRCrash tx p)
+Definition do_tbegin (cc:tprog -> pprog) rx : pprog :=
+   tx <- PGetTx;
+   if tx then 
+    cc (rx TRFail)
+   else
+    PSetTx true ;; PClrLog ;; cc (rx TRSucc)
+.
+
+Definition do_tread (cc:tprog -> pprog) b rx : pprog :=
+  tx <- PGetTx;
+  if tx then
+    l <- PGetLog;
+    match (pfind l b) with
+    | Some v => cc (rx (TRValue v))
+    | None   => v <- PRead b; cc (rx (TRValue v))
+    end
+  else
+    v <- PRead b; cc (rx (TRValue v))
+.
+
+Definition do_twrite (cc:tprog -> pprog) b v rx : pprog :=
+  tx <- PGetTx;
+  if tx then
+    PAddLog b v ;; cc (rx TRSucc)
+  else
+    PWrite b v;; cc (rx TRSucc)
+.
+
+Definition do_tend (cc:tprog -> pprog) rx : pprog :=
+  tx <- PGetTx;
+  if tx then 
+    PSetTx false ;; l <- PGetLog ; pflush l ;; PClrLog ;; cc (rx TRSucc)
+  else
+    cc (rx TRFail)
+.
+
+Definition do_trecover rx : pprog :=
+  tx <- PGetTx;
+  if tx then
+    PClrLog ;; rx
+  else
+    l <- PGetLog; pflush l ;; rx
+.
+
+Close Scope pprog_scope.
+
+Fixpoint compile_tp (p:tprog) : pprog :=
+  match p with
+  | THalt         => PHalt
+  | TBegin rx     => do_tbegin compile_tp rx
+  | TRead b rx    => do_tread  compile_tp b rx
+  | TWrite b v rx => do_twrite compile_tp b v rx
+  | TEnd rx       => do_tend   compile_tp rx
+  end.
+
+Fixpoint pexec (p:pprog) (s:pstate) : pstate :=
+  let (d, l, c) := s in
+  match p with
+  | PHalt           => s
+  | PRead b rx      => pexec (rx (st_read d b)) (PSt d l c)
+  | PWrite b v rx   => pexec rx (PSt (st_write d b v) l c)
+  | PAddLog b v rx  => pexec rx (PSt d (l ++ [(b, v)]) c)
+  | PClrLog rx      => pexec rx (PSt d nil c)
+  | PGetLog rx      => pexec (rx l) (PSt d l c)
+  | PSetTx v rx     => pexec rx (PSt d l v)
+  | PGetTx rx       => pexec (rx c) (PSt d l c)
+  end.
+
+Inductive pstep : pstate -> pprog -> pstate -> Prop :=
+  | PsHalt: forall s,
+    pstep s PHalt s
+  | PsRead: forall d l c b rx s,
+    pstep (PSt d l c) (rx (st_read d b)) s ->
+    pstep (PSt d l c) (PRead b rx) s
+  | PsWrite: forall d l c b v rx s,
+    pstep (PSt (st_write d b v) l c) rx s ->
+    pstep (PSt d l c) (PWrite b v rx) s
+  | PsAddLog: forall d l c b v rx s,
+    pstep (PSt d (l ++ [(b, v)]) c) rx s ->
+    pstep (PSt d l c) (PAddLog b v rx) s
+  | PsClrLog: forall d l c rx s,
+    pstep (PSt d nil c) rx s ->
+    pstep (PSt d l c) (PClrLog rx) s
+  | PsGetLog: forall d l c rx s,
+    pstep (PSt d l c) (rx l) s ->
+    pstep (PSt d l c) (PGetLog rx) s
+  | PsSetTx: forall d l c v rx s,
+    pstep (PSt d l v) rx s ->
+    pstep (PSt d l c) (PSetTx v rx) s
+  | PsGetTx: forall d l c rx s,
+    pstep (PSt d l c) (rx c) s ->
+    pstep (PSt d l c) (PGetTx rx) s
+  | PsCrash: forall p s,
+    pstep s p (pexec (do_trecover PHalt) s)
+    (* XXX: how to continue running after recovery ? *)
   .
 
-Definition TInit := mkTState st_init TRNone false nil.
-
-(* low-level language *)
-
-Inductive LLOp : Set :=
-  | Read: storage -> block -> value -> LLOp
-  | Write: storage -> block -> value -> storage -> LLOp.
-
-Definition LLProg := list LLOp.
-
-Record LLState: Set := mkLLState {
-  logdisk : storage;
-  datadisk : storage
-}.
-
-(*
-
-Note: Since our target language is non-deterministic, 
-      we need to show backward simulation 
-
-XXX:  "plus" rule does not work well backwards, since
-      one high level step usually maps to multiple
-      low-level steps, but not the reverse.
-
-Lemma forward_sim:
-  forall h1 h2, Tstep h1 h2 ->
-  forall l1, match_states h1 l1 ->
-  exists l2, plus LLstep l1 l2 /\ match_states h2 l2.
 
 
-Lemma backward_sim:
-  forall l1 l2, LLstep l1 l2 ->
-  forall h1, match_states h1 l1 ->
-  exists h2, Tstep h1 h2 /\ match_states h2 l2.
-*)
+Fixpoint log_flush (p:list (block*value)) (d:storage) : storage :=
+  match p with
+  | nil            => d
+  | (b, v) :: rest => log_flush rest (st_write d b v)
+  end.
+
+Theorem correct' : forall d p l d' l' c',
+  pstep (PSt d l false) (compile_tp p) (PSt d' l' c')
+  -> d' = d \/ d' = TSDisk (texec p (TSt (log_flush l d) None)).
+Proof.
+  induction p; intros; auto.
+Admitted.
+
+(** Main correctness theorem *)
+Theorem correct : forall d p d' l' c',
+  pstep (PSt d nil false) (compile_tp p) (PSt d' l' c')
+  -> d' = d \/ d' = TSDisk (texec p (TSt d None)).
+Proof.
+  intros. apply correct' in H. auto.
+Qed.
